multiset order specialized to worklist algorithms

src/num/termination/TotalDefn.sml
@@ -152,6 +152,7 @@ val termination_simps =
           prim_recTheory.measure_def,
           relationTheory.inv_image_def,
           pairTheory.LEX_DEF,
+          pairTheory.RPROD_DEF,
           SUB_LESS_I,DIV_LESS_I,MOD_LESS_I];
 
 (*---------------------------------------------------------------------------*)
